assign 12

assignments/12/P10.v
@@ -4,21 +4,63 @@ Require Export P09.
 
 (** Write a type inference function [tyeq: tm -> option ty].
 **)
+Print tm. 
+Print ty.
+
 
 Fixpoint tyinfer (t: tm) : option ty :=
-  GIVEUP.
+    match t with
+    | ttrue => Some TBool
+    | tfalse => Some TBool
+    | tif t1 t2 t3 => match (tyinfer t1) with 
+                | Some TBool => match (tyinfer t2) with
+                                | Some TBool => match (tyinfer t3) with
+                                    |Some TBool => Some TBool
+                                    |Some TNat => None
+                                    | None => None
+                                    end
+                                | Some TNat => match (tyinfer t3) with
+                                    |Some TBool => None
+                                    | Some TNat => Some TNat
+                                    | None => None
+                                    end
+                                | None => None
+                                end
+                | Some TNat => None
+                | None => None
+                end
+    | tzero => Some TNat
+    | tsucc t => match (tyinfer t) with
+                | Some TBool => None
+                | Some TNat => Some TNat
+                | None => None
+                end
+    | tpred t => match (tyinfer t) with
+                | Some TBool => None
+                | Some TNat => Some TNat
+                | None => None
+                end
+    | tiszero t => match (tyinfer t) with
+                | Some TBool => None
+                | Some TNat => Some TBool
+                | None => None
+                end
+    
+    end.
+
+
 
 Example tyinfer_ex1:
   tyinfer
     (tif (tiszero (tpred (tsucc (tsucc tzero)))) ttrue (tiszero (tsucc tzero))) 
   = Some TBool.
-Proof. exact GIVEUP. Qed.
+Proof. reflexivity. Qed.
 
 Example tyinfer_ex2:
   tyinfer
     (tif (tiszero (tpred (tsucc (tsucc tzero)))) tzero (tiszero (tsucc tzero))) 
   = None.
-Proof. exact GIVEUP. Qed.
+Proof. reflexivity. Qed.
 
 (** Prove that the type checking function [tyeq: tm -> ty -> bool] is correct.
 
@@ -31,13 +73,39 @@ Theorem tyinfer_correct1: forall t T
     (TYCHK: tyinfer t = Some T),
   |- t \in T.
 Proof.
-  exact GIVEUP.
+  exact GIVEUP. 
+
+
+
 Qed.
 
 Theorem tyinfer_correct2: forall t T
     (HASTY: |- t \in T),
   tyinfer t = Some T.
 Proof.
-  exact GIVEUP.
+  intros.
+  generalize dependent T.
+  induction t; intros.
+  - inversion T; inversion HASTY. auto. auto. 
+  - inversion T; inversion HASTY. auto. auto.
+  - inversion T; inversion HASTY; subst. apply IHt1 in H2.
+    apply IHt2 in H4. apply IHt3 in H5. simpl.  rewrite H2. rewrite H4.
+    rewrite H5. auto.  eauto.  destruct T.  reflexivity. reflexivity.
+    apply IHt1 in H2. apply IHt2 in H4. apply IHt3 in H5.
+    simpl. rewrite H2. rewrite H4. rewrite H5. destruct T. 
+    reflexivity. reflexivity.
+  - inversion T; inversion HASTY. auto. auto. 
+  - inversion T; inversion HASTY. apply IHt in H0. simpl. 
+    rewrite H0. reflexivity.
+    apply IHt in H0. simpl. rewrite H0. reflexivity.
+  -  inversion T; inversion HASTY. apply IHt in H0. simpl. 
+    rewrite H0. reflexivity.
+    apply IHt in H0. simpl. rewrite H0. reflexivity.
+  -  inversion T; inversion HASTY. apply IHt in H0. simpl. 
+    rewrite H0. reflexivity.
+    apply IHt in H0. simpl. rewrite H0. reflexivity.  
+
+
+
 Qed.
 
