assignments/12/P01.v
@@ -6,6 +6,17 @@ Require Export D.
 Example some_term_is_stuck :
   exists t, stuck t.
 Proof.
-  exact GIVEUP.
+  unfold stuck.
+  intros. unfold not.
+  Print tm.
+  exists (tsucc ttrue).
+  split.
+  Print step_normal_form.
+    unfold normal_form. unfold not.
+    intros. inversion H; subst. inversion H0. subst. 
+    inversion H2.
+    intros.
+    inversion H;subst. inversion H0. inversion H0; subst.
+    inversion H2. 
 Qed.
 
