assignments/12/P03.v
@@ -9,6 +9,36 @@ Require Export P02.
 Theorem step_deterministic:
   deterministic step.
 Proof with eauto.
-  exact GIVEUP.
+    unfold deterministic.
+  intros. generalize dependent y2.
+  step_cases (induction H) Case; subst; intros.
+-  inversion H0. reflexivity. 
+  solve by inversion. 
+-
+  inversion H0. reflexivity.
+  solve by inversion.
+- inversion H0; subst. solve by inversion.
+  solve by inversion.
+  f_equal.   auto. 
+- inversion H0. subst. f_equal.  auto. 
+- inversion H0. reflexivity. inversion H1. 
+- inversion H0. subst. reflexivity.
+  assert (value t1). right. assumption.
+  apply value_is_nf in H4. unfold normal_form, not in H4.
+  inversion H2; subst. exfalso. apply H4. exists t1'0. assumption. 
+- inversion H0; subst; try (solve by inversion).
+  assert (value y2). right. assumption.
+  apply value_is_nf in H1. unfold normal_form, not in H1.
+  inversion H; subst. exfalso. apply H1. exists t1'0. assumption.
+  apply IHstep in H2. rewrite H2. reflexivity.
+- inversion H0; subst. reflexivity. solve by inversion.
+- inversion H0; subst. reflexivity.
+  assert (value t1). right. assumption. apply value_is_nf in H1.
+  unfold normal_form, not in H1.
+  inversion H2; subst. exfalso. apply H1. exists t1'0. assumption.
+- inversion H0; subst; try (solve by inversion). 
+  assert (value t0). right. assumption. apply value_is_nf in H1. 
+  unfold normal_form, not in H1.
+  inversion H; subst. exfalso. apply H1. exists t1'0. assumption. 
+  rewrite (IHstep t1'0). reflexivity. assumption. 
 Qed.
-
