assignments/12/P04.v
@@ -7,6 +7,8 @@ Example succ_hastype_nat__hastype_nat : forall t,
   |- tsucc t \in TNat ->
   |- t \in TNat.  
 Proof.
-  exact GIVEUP.
+  intros.
+  inversion H; subst.
+  assumption.
 Qed.
 
